test/dafny/merkle/third_party_implementations/ThirdPartyMerkleisation.dfy
@@ -19,4 +19,5 @@ module {:extern "thirdpartymerkleisation"} ThirdPartyMerkleisation {
     import opened Eth2Types
     import opened NativeTypes
     function method {:extern} BitlistRoot(rbl: seq<bool>, brbl:seq<byte>, limit:nat): hash32
+    function method {:extern} BytesRoot(bs: seq<byte>): hash32
 }
